thy/Iptables_Semantics/Primitive_Matchers/Output_Interface_Replace.thy
@@ -174,7 +174,8 @@ begin
        "normalized_nnf_match m \<Longrightarrow> ipassmt_sanity_nowildcards ipassmt (*TODO: check?*) \<Longrightarrow>
         correct_routing rt \<Longrightarrow>
         ipassmt = map_of (routing_ipassmt rt ifs) \<Longrightarrow>
-        output_iface (routing_table_semantics rt (p_dst p)) = p_oiface p \<Longrightarrow>
+        routing_table_semantics rt (p_dst p) = Some ra \<Longrightarrow>
+        output_iface ra = p_oiface p \<Longrightarrow>
         matches (common_matcher, \<alpha>) (oiface_rewrite ipassmt m) a p \<longleftrightarrow> matches (common_matcher, \<alpha>) m a p"
   apply(rule matches_oiface_rewrite_ipassmt; assumption?)
    apply(simp add: correct_routing_def routing_ipassmt_ipassmt_sanity_disjoint; fail)
